examples/miniparse/MiniParseExample3.fst
@@ -1,0 +1,14 @@
+module MiniParseExample3
+open MiniParse.Tac.Spec
+open MiniParse.Tac.Impl
+open FStar.Tactics
+
+let ps' : package palette = _ by (gen_package Goal (`palette))
+
+let ps = ps'
+
+#set-options "--print_implicits --print_universes"
+
+let p' : parser_impl (package_parser ps') = _ by (gen_parser_impl Goal)
+
+let p = p'
