examples/miniparse/MiniParseExample3.fsti
@@ -1,0 +1,12 @@
+module MiniParseExample3
+open MiniParse.Tac.Spec
+open MiniParse.Impl.Base
+
+module U8 = FStar.UInt8
+
+type color = | Red | Blue | Green | Yellow
+type palette = nlist 18 U8.t // color // * U8.t)
+
+val ps: package palette
+
+val p: parser_impl (package_parser ps)
